src/simulation/Cert_rf.v
@@ -1,0 +1,731 @@
+From hahn Require Import Hahn.
+
+From imm Require Import Events.
+From imm Require Import Execution.
+From imm Require Import Execution_eco.
+From imm Require Import imm_bob imm_s_ppo.
+From imm Require Import imm_s_hb.
+From imm Require Import imm_s.
+From imm Require Import imm_common_more.
+From imm Require Import CertCOhelper.
+From imm Require Import CombRelations.
+
+Require Import AuxRel2.
+Require Import TraversalConfig.
+Require Import TraversalConfigAlt.
+Require Import TraversalConfigAltOld.
+Require Import ExtTraversalConfig.
+
+Require Import ImmProperties.
+
+Require Import Cert_co.
+Require Import Cert_D.
+
+Set Implicit Arguments.
+Remove Hints plus_n_O.
+
+Notation "'Tid_' t" := (fun x => tid x = t) (at level 1).
+Notation "'NTid_' t" := (fun x => tid x <> t) (at level 1).
+
+Section CertExec_rf.
+
+Variable G : execution.
+Variable sc : relation actid.
+
+Notation "'Init'" := (fun a => is_true (is_init a)).
+
+Notation "'E'" := G.(acts_set).
+Notation "'Gacts'" := G.(acts).
+Notation "'Glab'" := G.(lab).
+Notation "'Gsb'" := G.(sb).
+Notation "'Grf'" := G.(rf).
+Notation "'Gco'" := G.(co).
+Notation "'Grmw'" := G.(rmw).
+Notation "'Gdata'" := G.(data).
+Notation "'Gaddr'" := G.(addr).
+Notation "'Gctrl'" := G.(ctrl).
+Notation "'Gdeps'" := G.(deps).
+Notation "'Grmw_dep'" := G.(rmw_dep).
+
+Notation "'Gfre'" := G.(fre).
+Notation "'Grfe'" := G.(rfe).
+Notation "'Gcoe'" := G.(coe).
+Notation "'Grfi'" := G.(rfi).
+Notation "'Gfri'" := G.(fri).
+Notation "'Gcoi'" := G.(coi).
+Notation "'Gfr'" := G.(fr).
+Notation "'Geco'" := G.(eco).
+Notation "'Gdetour'" := G.(detour).
+Notation "'Gsw'" := G.(sw).
+Notation "'Grelease'" := G.(release).
+Notation "'Grs'" := G.(rs).
+Notation "'Ghb'" := G.(hb).
+Notation "'Gppo'" := G.(ppo).
+Notation "'Grppo'" := G.(rppo).
+Notation "'Gbob'" := G.(bob).
+Notation "'Gfwbob'" := G.(fwbob).
+Notation "'Gar'" := (G.(ar) sc).
+Notation "'Gar_int'" := (G.(ar_int)).
+Notation "'Gurr'" := (G.(urr) sc).
+Notation "'Gfurr'" := (G.(furr) sc).
+Notation "'Gmsg_rel'" := (G.(msg_rel) sc).
+
+Notation "'Gloc'" := (loc Glab).
+Notation "'Gval'" := (val Glab).
+Notation "'Gsame_loc'" := (same_loc Glab).
+
+Notation "'R'" := (fun a => is_true (is_r Glab a)).
+Notation "'W'" := (fun a => is_true (is_w Glab a)).
+Notation "'F'" := (fun a => is_true (is_f Glab a)).
+Notation "'GR_ex'" := (fun a => is_true (R_ex Glab a)).
+Notation "'GW_ex'" := G.(W_ex).
+Notation "'GW_ex_acq'" := (GW_ex ∩₁ (fun a => is_true (is_xacq Glab a))).
+
+Notation "'Loc_' l" := (fun x => Gloc x = Some l) (at level 1).
+Notation "'W_' l" := (W ∩₁ Loc_ l) (at level 1).
+Notation "'R_' l" := (R ∩₁ Loc_ l) (at level 1).
+
+Notation "'Pln'" := (fun a => is_true (is_only_pln Glab a)).
+Notation "'Rlx'" := (fun a => is_true (is_rlx Glab a)).
+Notation "'Rel'" := (fun a => is_true (is_rel Glab a)).
+Notation "'Acq'" := (fun a => is_true (is_acq Glab a)).
+Notation "'Acqrel'" := (fun a => is_true (is_acqrel Glab a)).
+Notation "'Acq/Rel'" := (fun a => is_true (is_ra Glab a)).
+Notation "'Sc'" := (fun a => is_true (is_sc Glab a)).
+Notation "'xacq'" := (fun a => is_true (is_xacq Glab a)).
+
+
+Variable T : trav_config.
+Variable S : actid -> Prop.
+
+Notation "'I'" := (issued T).
+Notation "'C'" := (covered T).
+
+Variable thread : BinNums.positive.
+
+Notation "'cert_co'" := (cert_co G T thread).
+
+Notation "'D'" := (D G T S thread).
+
+
+Hypothesis WF : Wf G.
+Hypothesis WF_SC : wf_sc G sc.
+Hypothesis RELCOV : W ∩₁ Rel ∩₁ I ⊆₁ C.
+Hypothesis TCCOH : tc_coherent G sc T.
+Hypothesis ACYC_EXT : acyc_ext G sc.
+Hypothesis CSC : coh_sc G sc.
+Hypothesis COH : coherence G.
+Hypothesis AT : rmw_atomicity G.
+
+Hypothesis IT_new_co: I ∪₁ E ∩₁ W ∩₁ Tid_ thread ≡₁ E ∩₁ W.
+Hypothesis E_to_S: E ⊆₁ C ∪₁ dom_rel (Gsb^? ⨾ ⦗S⦘).
+Hypothesis Grfe_E : dom_rel Grfe ⊆₁ I.
+Hypothesis E_F_AcqRel_in_C: E ∩₁ F ∩₁ Acq/Rel ⊆₁ C.
+Hypothesis COMP_ACQ: forall r (IN: (E ∩₁ R ∩₁ Acq) r), exists w, Grf w r.
+Hypothesis urr_helper: dom_rel ((Ghb ⨾ ⦗F ∩₁ Sc⦘)^? ⨾ sc^? ⨾ Ghb^? ⨾ Grelease ⨾ ⦗I⦘) ⊆₁ C.
+Hypothesis urr_helper_C: dom_rel ((Ghb ⨾ ⦗F ∩₁ Sc⦘)^? ⨾ sc^? ⨾ Ghb^? ⨾ (Grelease ⨾ Grf)^? ⨾ ⦗C⦘) ⊆₁ C.
+Hypothesis W_hb_sc_hb_to_I_NTid: dom_rel (⦗W⦘ ⨾ Ghb ⨾ (sc ⨾ Ghb)^? ⨾ ⦗I ∩₁ NTid_ thread⦘) ⊆₁ I.
+Hypothesis detour_E : dom_rel (Gdetour ⨾ ⦗E ∩₁ NTid_ thread⦘) ⊆₁ I.
+Hypothesis detour_Acq_E : dom_rel (Gdetour ⨾ ⦗E ∩₁ R ∩₁ Acq⦘) ⊆₁ I.
+Hypothesis hb_sc_hb_de : ⦗(E \₁ C) ∩₁ (E \₁ I)⦘ ⨾ Ghb ⨾ (sc ⨾ Ghb)^? ⊆ Gsb.
+Hypothesis COMP_C : C ∩₁ R ⊆₁ codom_rel Grf.
+Hypothesis COMP_NTID : E ∩₁ NTid_ thread ∩₁ R ⊆₁ codom_rel Grf.
+Hypothesis COMP_PPO : dom_rel (Gppo ⨾ ⦗I⦘) ⊆₁ codom_rel Grf.
+Hypothesis COMP_RPPO : dom_rel (⦗R⦘ ⨾ (Gdata ∪ Grfi ∪ Grmw)＊ ⨾ Grppo ⨾ ⦗S⦘) ⊆₁ codom_rel Grf.
+Hypothesis TCCOH_rst_new_T : tc_coherent G sc (mkTC (C ∪₁ (E ∩₁ NTid_ thread)) I).
+
+Hypothesis S_in_W : S ⊆₁ W.
+Hypothesis RPPO_S : dom_rel ((Gdetour ∪ Grfe) ⨾ (Gdata ∪ Grfi ∪ Grmw)＊ ⨾ Grppo ⨾ ⦗S⦘) ⊆₁ I.
+Hypothesis ST_in_E : S ∩₁ Tid_ thread ⊆₁ E.
+Hypothesis I_in_S : I ⊆₁ S.
+Hypothesis W_ex_acq_in_I :GW_ex_acq ⊆₁ I.
+
+Hypothesis F_in_C : E ∩₁ F ∩₁ Acq/Rel ⊆₁ C.
+
+Hypothesis S_I_in_W_ex : (S ∩₁ Tid_ thread) \₁ I ⊆₁ W_ex G.
+
+Hypothesis ETC_DR_R_ACQ_I : dom_rel ((Gdetour ∪ Grfe) ⨾ (Grmw ⨾ Grfi)^* ⨾ ⦗R∩₁Acq⦘ ⨾ Gsb ⨾ ⦗S⦘) ⊆₁ I.
+
+Hypothesis COMP_R_ACQ_SB : dom_rel ((Grmw ⨾ Grfi)＊ ⨾ ⦗E ∩₁ R ∩₁ Acq⦘) ⊆₁ codom_rel Grf.
+
+
+(******************************************************************************)
+(** Definition of the new rf edges   *)
+(******************************************************************************)
+
+Definition new_rf := Gfurr ∩ Gsame_loc ⨾ ⦗(E \₁ D) ∩₁ R⦘ \ cert_co ⨾ Gfurr.
+
+Lemma wf_new_rfE : new_rf ≡ ⦗E⦘ ⨾ new_rf ⨾ ⦗E \₁ D⦘.
+Proof using WF WF_SC.
+apply dom_helper_3.
+unfold new_rf.
+rewrite (wf_furrE WF WF_SC); basic_solver 21.
+Qed.
+
+Lemma wf_new_rfD : new_rf ≡ ⦗W⦘ ⨾ new_rf ⨾ ⦗R⦘.
+Proof using.
+apply dom_helper_3.
+unfold new_rf.
+unfold furr, urr; basic_solver.
+Qed.
+
+Lemma wf_new_rfl : new_rf ⊆ Gsame_loc.
+Proof using.
+unfold new_rf; basic_solver.
+Qed.
+
+Lemma wf_new_rff : functional new_rf⁻¹.
+Proof using WF WF_SC IT_new_co ST_in_E S_in_W.
+  rewrite wf_new_rfD, wf_new_rfE.
+  red; ins.
+  assert (exists l, Gloc y = Some l).
+  { generalize (is_w_loc Glab). generalize H. basic_solver 12. }
+  desc.
+
+  assert (Gloc z = Some l).
+  { hahn_rewrite wf_new_rfl in H; hahn_rewrite wf_new_rfl in H0.
+    generalize H H0. unfolder. ins. desf. congruence. }
+  unfolder in H. unfolder in H0.
+  destruct (classic (y=z)) as [|X]; eauto; desf.
+  exfalso. eapply wf_cert_co_total in X; try edone.
+  unfold new_rf in *. desf.
+  all: unfolder in H12; unfolder in H5; basic_solver 40.
+Qed.
+
+Lemma new_rf_comp : forall b (IN: ((E \₁ D) ∩₁ R) b) , exists a, new_rf a b.
+Proof using WF WF_SC IT_new_co ST_in_E S_in_W.
+  ins; unfolder in IN; desf.
+  assert (exists l, Gloc b = Some l); desc.
+  { generalize (is_r_loc Glab). basic_solver 12. }
+  assert (E (InitEvent l)).
+  { apply WF; eauto. }
+  assert (Glab (InitEvent l) = Astore Xpln Opln l 0) by apply WF. 
+  assert (Gloc (InitEvent l) = Some l).
+  { unfold loc. by rewrite (wf_init_lab WF). }
+  assert (W_ l (InitEvent l)).
+  { unfolder. unfold is_w, loc; desf; eauto. }
+  assert (Gsb (InitEvent l) b).
+  { apply init_ninit_sb; eauto. eapply read_or_fence_is_not_init; eauto. }
+  assert (Gurr l (InitEvent l) b).
+  { exists (InitEvent l); splits.
+    unfold eqv_rel; eauto.
+    hahn_rewrite <- sb_in_hb.
+    basic_solver 12. }
+
+  forward (eapply last_exists with (s:=cert_co ⨾ ⦗fun x=> Gfurr x b⦘) 
+                                   (dom:= filterP (W_ l) G.(acts)) (a:=(InitEvent l))).
+  { eapply acyclic_mon.
+    apply trans_irr_acyclic; [eapply cert_co_irr| eapply cert_co_trans]; try edone.
+    basic_solver. }
+  { ins.
+    assert (A: (cert_co ⨾ ⦗fun x : actid => Gfurr x b⦘)^? (InitEvent l) c).
+    { apply rt_of_trans; try done.
+      apply transitiveI; unfolder; ins; desf; splits; eauto.
+      eapply cert_co_trans; eauto. }
+    unfolder in A; desf.
+    { apply in_filterP_iff; split; auto. }
+    apply in_filterP_iff.
+    eapply wf_cert_coE in A; try edone.
+    unfolder in A; desc.
+    eapply wf_cert_coD in A1; try edone.
+    unfolder in A1; desc.
+    eapply wf_cert_col in A3; try edone.
+    unfold same_loc in *.
+    unfolder in A.
+    desf; splits; eauto. red. splits; auto.
+    congruence. }
+  ins; desf.
+  assert (A: (cert_co ⨾ ⦗fun x : actid => Gfurr x b⦘)^? (InitEvent l) b0).
+  { apply rt_of_trans; try done.
+    apply transitiveI; unfolder; ins; desf; splits; eauto.
+    eapply cert_co_trans; eauto. }
+  assert (Gloc b0 = Some l).
+  { unfolder in A; desf.
+    eapply wf_cert_col in A; try edone.
+    unfold same_loc in *; desf. unfolder in H7; congruence. }
+  exists b0; red; split.
+  { unfold furr, same_loc.
+    unfolder in A; desf.
+    all: unfolder; ins; desf.
+    all: splits; try congruence.
+    all: basic_solver 21. }
+  unfold max_elt in *.
+  unfolder in H7; ins; desf; intro; desf.
+  unfolder in H9. desf.
+  eapply H7. eauto.
+Qed.
+
+Lemma new_rf_mod: (E \₁ D) ∩₁ is_r Glab ≡₁ codom_rel new_rf.
+Proof using WF WF_SC IT_new_co ST_in_E S_in_W.
+  split.
+  unfolder; ins; desf.
+  apply new_rf_comp; basic_solver.
+  unfold new_rf; basic_solver.
+Qed.
+
+Lemma new_rf_in_furr: new_rf ⊆ Gfurr.
+Proof using.
+unfold new_rf; basic_solver.
+Qed.
+
+Lemma new_rf_hb: irreflexive (new_rf ⨾ Ghb ⨾ (sc ⨾ Ghb)^?).
+Proof using WF WF_SC CSC COH ACYC_EXT.
+rewrite new_rf_in_furr.
+apply furr_hb_sc_hb_irr; done.
+Qed.
+
+Lemma non_I_new_rf: ⦗E \₁ I⦘ ⨾ new_rf ⊆ Gsb.
+Proof using WF WF_SC CSC COH ACYC_EXT IT_new_co.
+  assert (new_rf_hb: irreflexive (new_rf ⨾ Ghb ⨾ (sc ⨾ Ghb)^?)).
+  { by apply new_rf_hb. (* Coq bug ?! *) }
+
+  rewrite wf_new_rfD.
+  arewrite (⦗E \₁ I⦘ ⨾ ⦗W⦘ ⊆ ⦗E \₁ I⦘ ⨾ ⦗Tid_ thread⦘ ⨾ ⦗W⦘).
+  { rewrite <- id_inter at 1.
+    rewrite set_inter_minus_l.
+    rewrite <- IT_new_co.
+    clear.
+    basic_solver. }
+  rewrite wf_new_rfE.
+  arewrite (E \₁ D ⊆₁ E ∩₁ Tid_ thread).
+  { unfold Cert_D.D. clear. unfolder. ins. desf; tauto. }
+  clear -new_rf_hb WF.
+  unfolder; ins; desf.
+  eapply (@same_thread G) in H3; desf.
+  destruct H3; [subst x; type_solver|].
+  2: intro K; apply (init_w WF) in K; type_solver.
+  exfalso. generalize new_rf_hb.
+  generalize (@sb_in_hb G).
+  basic_solver 12.
+Qed.
+
+Lemma non_S_new_rf: ⦗E \₁ S⦘ ⨾ new_rf ⊆ Gsb.
+Proof using WF WF_SC CSC COH ACYC_EXT IT_new_co I_in_S.
+  rewrite <- I_in_S.
+  apply non_I_new_rf.
+Qed.
+
+Lemma new_rfe_Acq : (new_rf \ Gsb) ⨾ ⦗R∩₁Acq⦘ ⊆ ∅₂.
+Proof using WF WF_SC ACYC_EXT COH COMP_ACQ CSC IT_new_co S ST_in_E S_in_W.
+rewrite wf_new_rfE.
+arewrite (⦗E⦘ ⊆ ⦗E \₁ I⦘ ∪ ⦗E ∩₁ I⦘).
+unfolder; ins; desf; tauto.
+relsf.
+rewrite minus_union_l.
+relsf; unionL.
+sin_rewrite non_I_new_rf.
+basic_solver.
+rewrite wf_new_rfD.
+arewrite (new_rf ⊆ new_rf ∩ Gsame_loc).
+generalize (wf_new_rfl); basic_solver.
+
+unfolder; ins; desf.
+
+assert (Lx:exists l, Gloc x = Some l); desc.
+by apply is_w_loc.
+
+assert (Ly:Gloc y = Some l).
+unfold same_loc in *; congruence.
+
+forward (apply COMP_ACQ).
+by basic_solver.
+
+ins; desc.
+
+apply rfi_union_rfe in H10; unfolder in H10; desf; cycle 1.
+by generalize R_Acq_codom_rfe; basic_solver 12.
+
+ie_unfolder; unfolder in H10; desf.
+
+hahn_rewrite (wf_rfD WF) in H10.
+hahn_rewrite (wf_rfE WF) in H10.
+
+unfolder in H10; desf.
+
+assert (Lz:Gloc z = Some l).
+by apply (wf_rfl WF) in H14; unfold same_loc in *; congruence.
+
+forward (apply ((wf_co_total WF) (Some l) z)).
+basic_solver.
+instantiate (1 := x).
+basic_solver.
+
+intro; desf.
+
+intro; desf.
+
+- eapply eco_furr_irr; try edone.
+  eexists; splits; [|eby apply new_rf_in_furr].
+  unfold eco, fr.
+  basic_solver 12.
+- eapply H3.
+  exists z; split; [| apply furr_alt; basic_solver 12].
+  eapply I_co_in_cert_co; try edone.
+  apply seq_eqv_l. split; auto.
+  red. basic_solver.
+Qed.
+
+Lemma dom_Grfi_nD_in_thread :
+  dom_rel (Grfi ⨾ ⦗set_compl D⦘) ⊆₁ Tid_ thread.
+Proof using WF TCCOH.
+  unfolder. intros x [y [RFI ND]].
+  destruct (classic (I x)) as [IX|NIX].
+  { exfalso. apply ND.
+    do 2 red. left. left. right. basic_solver 10. }
+  destruct RFI as [RF SB].
+  apply WF.(wf_rfE) in RF.
+  unfolder in RF. desf.
+  assert (~ is_init x) as NINX.
+  { intros II. apply NIX. 
+    eapply init_issued; eauto. by split. }
+  apply sb_tid_init in SB. desf.
+  apply NNPP. intros NTX.
+  assert (tid y <> thread) as NTY.
+  { intros HH. apply NTX. by rewrite <- HH. }
+  apply ND. red. do 5 left. right. by split.
+Qed.
+
+Lemma Grfi_nD_in_new_rf : Grfi ⨾ ⦗set_compl D⦘ ⊆ new_rf.
+Proof using All.
+  unfold new_rf.
+  rewrite AuxRel.minus_inter_compl.
+  apply inclusion_inter_r.
+  { rewrite furr_alt; [|done].
+    arewrite (Grfi ⊆ Grf).
+    rewrite (dom_r WF.(wf_rfE)) at 1.
+    rewrite (WF.(wf_rfD)) at 1.
+    arewrite (Grf ⊆ Grf ∩ Grf) at 1.
+    rewrite (WF.(wf_rfl)) at 1.
+    clear.
+    basic_solver 21. }
+  rewrite (dom_rel_helper dom_Grfi_nD_in_thread).
+  arewrite (Grfi ⊆ Grf).
+  rewrite cert_co_alt'; try edone.
+  unfolder; ins; desf.
+  intro; desf.
+  eapply eco_furr_irr; try edone.
+  exists z; splits; eauto.
+  red; right. unfolder; ins; desf.
+  exists z; splits; eauto; red.
+  basic_solver.
+Qed.
+
+(******************************************************************************)
+(** Definition of certification graph rf relation   *)
+(******************************************************************************)
+
+Definition Crf := Grf ⨾ ⦗D⦘ ∪ new_rf.
+Definition Crfe := Crf \ Gsb.
+Definition Crfi := Crf ∩ Gsb.
+
+Lemma cert_rfe : Crfe ≡ ⦗I⦘ ⨾ Grfe ⨾ ⦗D⦘ ∪ ⦗I⦘ ⨾ (new_rf \ Gsb).
+Proof using WF WF_SC ACYC_EXT COH CSC IT_new_co Grfe_E.
+unfold Execution.rfe, Crfe, Crf.
+split; [|basic_solver 12].
+rewrite minus_union_l; unionL.
+generalize Grfe_E; ie_unfolder; basic_solver 21.
+rewrite wf_new_rfE at 1; try edone.
+arewrite (⦗E⦘ ⊆ ⦗E ∩₁ I⦘ ∪ ⦗E \₁ I⦘) at 1.
+  by unfolder; ins; desf; tauto.
+relsf; rewrite minus_union_l; unionL.
+basic_solver 21.
+rewrite <- seqA.
+rewrite (non_I_new_rf); try edone.
+basic_solver 21.
+Qed.
+
+Lemma cert_rfe_D : Crfe ⨾ ⦗D⦘ ⊆ ⦗I⦘ ⨾ Grfe.
+Proof using WF WF_SC ACYC_EXT COH CSC IT_new_co Grfe_E.
+rewrite cert_rfe.
+rewrite (dom_r wf_new_rfE).
+basic_solver 12.
+Qed.
+
+Lemma cert_rf_D : Crf ⨾ ⦗D⦘ ≡ Grf ⨾ ⦗D⦘.
+Proof using WF WF_SC.
+  unfold Crf.
+  ins; split; [rewrite wf_new_rfE|].
+  all: clear; basic_solver 20.
+Qed.
+
+Lemma dom_rf_D_helper: Grf ⨾ ⦗D⦘ ≡ ⦗D⦘ ;; Grf ⨾ ⦗D⦘.
+Proof.
+forward (eapply dom_rf_D with (T:=T) (S:=S) (thread:=thread)); try edone.
+basic_solver 12.
+Qed.
+
+Lemma cert_rfi_D : Crfi ⨾ ⦗D⦘ ⊆ ⦗D⦘ ⨾ Grfi ⨾ ⦗D⦘.
+Proof using  WF WF_SC TCCOH Grfe_E.
+unfold Crfi, Crf.
+rewrite <- seq_eqv_inter_lr.
+seq_rewrite cert_rf_D. 
+rewrite dom_rf_D_helper.
+clear.
+basic_solver 12.
+Qed.
+
+Lemma dom_Crfe_in_I: dom_rel Crfe ⊆₁ I.
+Proof using All.
+  (* HINT: use Lemma non_I_new_rf: ⦗E \₁ I⦘ ⨾ new_rf ⊆ Gsb. *)
+Admitted.
+
+Lemma Grfi_in_Crfi : Grfi ⊆ Crfi.
+Proof using All.
+arewrite (Grfi ⊆ Grfi ⨾ ⦗D ∪₁ set_compl D⦘).
+by clear; unfolder; ins; desf; tauto.
+rewrite id_union; rewrite seq_union_r; unionL.
+{ unfold rfi, Crfi, Crf.
+  generalize cert_rf_D.
+  by clear; unfolder; ins; desf; unfolder; eauto 12. }
+arewrite (Grfi ⨾ ⦗set_compl D⦘ ⊆ Gsb ∩ (Grfi ⨾ ⦗set_compl D⦘)).
+by clear; unfold rfi; basic_solver.
+rewrite Grfi_nD_in_new_rf. 
+unfold rfi, Crfi, Crf.
+clear; simpl; basic_solver.
+Qed.
+
+(* TODO: move to CombRelations.v *)
+Lemma rf_in_furr : Grf ⊆ Gfurr.
+Proof using WF.
+unfold furr, urr.
+do 2 rewrite (dom_l WF.(wf_rfD)).
+unfolder; ins; desc.
+apply is_w_loc in H1; desf.
+basic_solver 21.
+Qed.
+
+Lemma Crf_in_furr : Crf ⊆ Gfurr.
+Proof using WF.
+unfold Crf.
+rewrite new_rf_in_furr.
+rewrite rf_in_furr.
+basic_solver.
+Qed.
+
+Lemma Grfe_in_inv_Gco_cr_Crf : Grfe ⊆ (Gco^{-1})^? ;; Crf.
+Proof using All.
+arewrite (Grfe ⊆ Grfe ⨾ ⦗D ∪₁ set_compl D⦘).
+by clear; unfolder; ins; desf; tauto.
+rewrite id_union; rewrite seq_union_r; unionL.
+{ arewrite (Grfe ⊆ Grf).
+  rewrite <- cert_rf_D. 
+  basic_solver. }
+arewrite (Grfe ⨾ ⦗set_compl D⦘ ⊆ ((Gco ∪ Gco^{-1})^? ;; Crf) ∩ Grfe).
+{ 
+rewrite WF.(wf_rfeE).
+rewrite WF.(wf_rfeD).
+unfolder; ins; desf.
+splits; eauto.
+exploit new_rf_comp; unfolder; ins; splits; eauto.
+desf; exists a; splits; eauto.
+2: unfold Crf; basic_solver.
+assert (H44:=H4).
+eapply is_w_loc in H4; desc.
+assert (H11:=x1).
+apply wf_new_rfD in x1.
+unfolder in x1; desf.
+assert (H111:=x1).
+eapply is_w_loc in x1; desc.
+cut (x <> a -> Gco x a \/ Gco a x).
+tauto.
+eapply WF.(wf_co_total).
+unfolder; splits; eauto.
+unfolder; splits; eauto.
+apply wf_new_rfE in H11; unfolder in H11; desf.
+apply wf_new_rfl in H11; unfolder in H11; desf.
+unfold rfe in H0; unfolder in H0; desf.
+apply WF.(wf_rfl) in H0; unfolder in H0; desf.
+unfold same_loc in *; congruence. }
+rewrite crE at 1; relsf.
+rewrite !inter_union_l; unionL.
+1,3: basic_solver.
+transitivity (fun _ _ : actid => False); [|basic_solver].
+rewrite Crf_in_furr.
+clear - COH WF WF_SC CSC.
+unfold rfe.
+unfolder; ins; desf.
+eapply eco_furr_irr; eauto.
+eexists; splits; eauto.
+apply fr_in_eco; eexists; splits; eauto.
+Qed.
+
+Lemma I_Grfe_in_inv_Gco_cr_Crf : Grfe ⊆ (cert_co ∩ Gco^{-1})^? ;; Crf.
+Proof.
+rewrite (dom_rel_helper Grfe_E).
+arewrite (Grfe ⊆ Grfe ⨾ ⦗D ∪₁ set_compl D⦘).
+by clear; unfolder; ins; desf; tauto.
+rewrite id_union; rewrite !seq_union_r; unionL.
+by clear; unfold Crf, rfe; simpl; basic_solver 12.
+arewrite (Grfe ⊆ Grfe ∩ Grfe).
+rewrite Grfe_in_inv_Gco_cr_Crf at 1.
+rewrite !crE; relsf.
+rewrite !inter_union_l, seq_union_l, seq_union_r; unionL.
+by basic_solver.
+unionR right.
+rewrite WF.(wf_coE).
+rewrite WF.(wf_coD).
+arewrite (Gco ⊆ Gco ∩ Gsame_loc) at 1.
+{ generalize WF.(wf_col); basic_solver. }
+unfolder; ins; desf.
+edestruct is_w_loc; eauto.
+exists z0; splits; eauto 10.
+eapply tot_ex.
+{ apply wf_new_co_total.
+  eapply IST_new_co; try edone.
+  all: apply WF. }
+{ unfolder; eauto. }
+{ unfolder; eauto. }
+2: by intro; subst; eapply WF.(co_irr); eauto.
+unfold Crf in H3.
+unfolder in H3; desf.
+intro HH.
+apply H3.
+eexists; splits; eauto.
+apply rf_in_furr; unfold rfe in *; unfolder in H2; desf; eauto.
+Qed.
+
+Lemma Grf_to_Acq_S_in_Crf : Grf ;; <| dom_rel ((Grmw ⨾ Grfi)^* ⨾ ⦗R∩₁Acq⦘ ⨾ Gsb ⨾ ⦗S⦘) |> ⊆ Crf.
+Proof using All.
+  rewrite rfi_union_rfe at 1. rewrite seq_union_l. unionL.
+  { rewrite Grfi_in_Crfi. arewrite (Crfi ⊆ Crf). clear. basic_solver. }
+arewrite (Grfe ⊆ Grfe ⨾ ⦗D ∪₁ set_compl D⦘).
+by clear; unfolder; ins; desf; tauto.
+rewrite id_union; rewrite !seq_union_l, !seq_union_r; unionL.
+by clear; unfold Crf, rfe; simpl; basic_solver 12.
+(*unfold certG; simpl; unionR right.*)
+rewrite (dom_rel_helper Grfe_E).
+arewrite (⦗I⦘ ⨾ Grfe ⊆ (Grfe) ∩ (⦗I⦘ ⨾ Grfe)).
+sin_rewrite I_Grfe_in_inv_Gco_cr_Crf.
+rewrite crE.
+rewrite seq_union_l, !inter_union_l, !seq_union_l; unionL.
+by basic_solver.
+transitivity (fun _ _ : actid => False); [|basic_solver].
+arewrite (cert_co ∩ Gco⁻¹ ⊆ cert_co ∩ Gco⁻¹ ;; <|set_compl I|>).
+{ cut (codom_rel (cert_co ∩ Gco⁻¹) ⊆₁ set_compl I).
+  basic_solver 21.
+  rewrite cert_co_alt'; try edone. unfolder; ins; desf; eauto.
+  exfalso; eapply WF.(co_irr); eapply WF.(co_trans); eauto. }
+rewrite (dom_l WF.(wf_coE)) at 1.
+rewrite transp_seq; rels.
+rewrite AuxRel.seq_eqv_inter_rr, !seqA.
+seq_rewrite <- seq_eqv_inter_lr.
+rewrite !seqA.
+arewrite (Crf ⨾ ⦗set_compl D⦘ ⊆ new_rf).
+{ unfold Crf; ins; basic_solver. }
+arewrite (⦗E⦘ ⨾ ⦗set_compl I⦘ ⨾ new_rf ⊆ ⦗set_compl I⦘ ⨾ Gsb).
+{ generalize non_I_new_rf; basic_solver 22. }
+rewrite coi_union_coe, transp_union, inter_union_r; relsf.
+rewrite inter_union_l; relsf.
+unionL.
+{ rewrite (dom_l (@wf_sbE G)) at 1.
+  arewrite (⦗set_compl I⦘ ⨾ ⦗E⦘ ⊆ ⦗set_compl Init⦘).
+  { generalize init_issued; basic_solver 21. }
+  arewrite (⦗set_compl Init⦘ ⊆ ⦗set_compl Init⦘ ;; ⦗set_compl Init⦘).
+  { basic_solver. }
+  arewrite (Gcoi ⊆ Gsb).
+  rewrite ninit_sb_same_tid.
+  rewrite <- seqA.
+  rewrite <- !AuxRel.seq_eqv_inter_rr.
+  arewrite (Gsb⁻¹ ⨾ ⦗set_compl Init⦘ ⊆ same_tid).
+  { generalize (@ImmProperties.ninit_sb_same_tid G).
+    unfold same_tid; unfolder; clear; ins; desf; symmetry; eauto. }
+  arewrite (cert_co ∩ same_tid ⨾ same_tid ⊆ same_tid).
+  { clear; generalize (ImmProperties.same_tid_trans); basic_solver 21. }
+  generalize (rfe_n_same_tid WF COH).
+  basic_solver 21. }
+revert ETC_DR_R_ACQ_I; unfold detour; basic_solver 21.
+Qed.
+
+Lemma Crff : functional Crf⁻¹.
+Proof using All.
+  unfold Crf.
+  rewrite transp_union; apply functional_union.
+  by unfolder; ins; eapply (wf_rff WF); basic_solver.
+  by apply wf_new_rff.
+  by unfolder; ins; desf; apply wf_new_rfE in H0; unfolder in H0; basic_solver.
+Qed.
+
+Lemma Crfi_to_Grfe_in_Gdetour : Crfi ;; <| codom_rel Grfe |> ⊆ Gdetour.
+Proof.
+arewrite (Grfe ⊆ Grfe ∩ Grfe).
+rewrite I_Grfe_in_inv_Gco_cr_Crf at 1.
+unfolder; ins; desf.
+{ admit. }
+admit.
+Admitted.
+
+Lemma Crf_to_Acq_S_in_Grf : Crf ;; <| dom_rel ((Grmw ⨾ Grfi)^* ⨾ ⦗R∩₁Acq⦘ ⨾ Gsb ⨾ ⦗S⦘) |> ⊆ Grf.
+Proof using All.
+  remember (dom_rel ((Grmw ⨾ Grfi)＊ ⨾ ⦗R ∩₁ Acq⦘ ⨾ Gsb ⨾ ⦗S⦘)) as X.
+  arewrite (Crf ⨾ ⦗X⦘ ⊆ Crf ⨾ <| codom_rel Grf |> ⨾ ⦗X⦘).
+  { subst X.  rewrite (dom_l (@wf_sbE G)), !seqA.
+    arewrite (⦗R ∩₁ Acq⦘ ⨾ ⦗E⦘ ⊆ ⦗E ∩₁ R ∩₁ Acq⦘) by basic_solver.
+    generalize COMP_R_ACQ_SB.
+    basic_solver 21. }
+  unfolder. ins. desf.
+  assert (x0 = x); subst; auto.
+  eapply Crff; eauto. red.
+  eapply Grf_to_Acq_S_in_Crf.
+  apply seq_eqv_r. by splits.
+Qed.
+
+Lemma Crf_to_Acq_nC_in_Grf : Crf ;; <| dom_rel ((Grmw ⨾ Grfi)^* ⨾ ⦗E∩₁R∩₁Acq \₁ C⦘) |> ⊆ Grf.
+Proof using All.
+  arewrite (E∩₁R∩₁Acq \₁ C ⊆₁ R∩₁Acq ∩₁ dom_rel (Gsb ⨾ ⦗S⦘)).
+  2: { rewrite id_inter. rewrite <- !seqA. rewrite dom_rel_eqv_dom_rel.
+       rewrite !seqA. apply Crf_to_Acq_S_in_Grf. }
+  rewrite E_to_S.
+  rewrite crE, seq_union_l. rewrite S_in_W at 1.
+  clear. type_solver 20.
+Qed.
+
+Lemma Crfi_Grmw_in_Grfi_Grmw :
+    Crfi ⨾ Grmw ⨾ (Grfi ⨾ Grmw)＊ ⨾ Grfi ⨾ ⦗Acq \₁ C⦘ ⊆
+    Grfi ⨾ Grmw ⨾ (Grfi ⨾ Grmw)＊ ⨾ Grfi.
+Proof using All.
+  rewrite (dom_r WF.(wf_rfiE)) at 2.
+  rewrite E_to_S.
+  rewrite (dom_r WF.(wf_rfiD)) at 2. rewrite !seqA.
+  arewrite (⦗R⦘ ⨾ ⦗C ∪₁ dom_rel (Gsb^? ⨾ ⦗S⦘)⦘ ⨾ ⦗Acq \₁ C⦘ ⊆
+            ⦗dom_rel (Gsb ⨾ ⦗S⦘)⦘ ⨾ ⦗Acq⦘).
+  { generalize S_in_W. clear. 
+    ins. unfolder. ins. desf; splits; eauto.
+    exfalso. apply S_in_W in H5. type_solver 10. }
+  arewrite (Grmw ⨾ (Grfi ⨾ Grmw)＊ ⨾ Grfi ⨾ ⦗dom_rel (Gsb ⨾ ⦗S⦘)⦘ ⨾ ⦗Acq⦘ ⊆
+            ⦗dom_rel ((Grmw ⨾ Grfi)＊ ⨾ ⦗R ∩₁ Acq⦘ ⨾ Gsb ⨾ ⦗S⦘)⦘ ;; Grmw ⨾ (Grfi ⨾ Grmw)＊ ⨾ Grfi).
+  2: { hahn_frame.
+       unfold Crfi, rfi.
+       generalize Crf_to_Acq_S_in_Grf. basic_solver 20. }
+  seq_rewrite <- !rt_seq_swap. rewrite !seqA.
+  remember (Grmw ⨾ Grfi) as X.
+  rewrite (dom_r WF.(wf_rfiD)) at 1.
+  assert (Grmw ⨾ Grfi ⊆ X) as AA by (by subst X).
+  rewrite !seqA. sin_rewrite AA. seq_rewrite <- !ct_end.
+  rewrite <- inclusion_t_rt.
+  basic_solver 10.
+Qed.
+
+Lemma Crfi_Grmw_rt_in_Grfi_Grmw :
+    (Crfi ⨾ Grmw)＊ ⨾ Grfi ⨾ ⦗Acq \₁ C⦘ ⊆
+    (Grfi ⨾ Grmw)＊ ⨾ Grfi.
+Proof using All.
+  eapply rt_ind_left with (P:=fun r=> r ;; Grfi ;; ⦗Acq \₁ C⦘); eauto with hahn.
+  { rewrite rtE. basic_solver 12. }
+  intros k H.
+  arewrite (⦗Acq \₁ C⦘ ⊆ ⦗Acq \₁ C⦘ ;; ⦗Acq \₁ C⦘) by (clear; basic_solver).
+  sin_rewrite H. rewrite !seqA.
+  rewrite Crfi_Grmw_in_Grfi_Grmw.
+  rewrite <- !seqA. rewrite <- ct_begin. by rewrite inclusion_t_rt.
+Qed.
+
+(* TODO: move up *)
+Lemma Crf_to_Acq_in_Grf : Crf ;; <| dom_rel ((Grmw ⨾ Grfi)^* ⨾ ⦗Acq⦘) |> ⊆ Grf.
+Proof using All.
+Admitted.
+
+Lemma Crfi_to_Acq_in_Grf : Crfi ⨾ ⦗Acq⦘  ⊆ Grfi.
+Proof using All.
+Admitted.
+
+
+End CertExec_rf.
